\documentclass[11pt]{article}
\usepackage{amsmath}
\usepackage{amsfonts}
\usepackage{fancyvrb}
\usepackage{float}
\usepackage{graphicx}
\usepackage{bm}
\begin{document}

\title{APPM 5510 HW 5}
\author{Zane Jakobs}

\maketitle

\subsection*{1} Let $\bm{\Pi}_{i;j}$ be the Jacobian of the flow map $\Psi$ at time $i$ with respect to the initial condition at time $j$. Varying one parameter at a time, starting with $\bm{x}_0$, we have
\[
\begin{aligned}
\nabla J_1 \cdot \delta\bm{x}_0 &= \nabla J_0 \cdot \bm{x}_0 + \lambda^T\bm{\Pi}_{1;0} \cdot \bm{x}_0\\
&= 2(\bm{x}_0 - \bm{x}_b)^T\bm{B}_0^{-1}\cdot \delta\bm{x}_0 + 2 (\bm{x}_1 - \Psi(\bm{x}_0))^T\bm{B}_1^{-1}\Pi_{1;0}^T \cdot \delta\bm{x}_0 + 2(\bm{y}_0 - \bm{H}_0\bm{x}_0)^T\bm{R}_0^{-1}\bm{H}_0\cdot \delta\bm{x}_0
\end{aligned}
\]
and with $\bm{x}_1$, we get
\[
\begin{aligned}
\nabla J_1 \cdot \delta\bm{x}_1 &=  \nabla J_0 \cdot \delta\bm{x}_1 - \lambda^T \cdot\delta\bm{x}_1\\
&= 2(\bm{x}_1 - \Psi(\bm{x}_0))^T\bm{B}_1^{-1} \cdot\delta\bm{x}_1 + 2(\bm{y}_1 - \bm{H}_1\bm{x}_1)^T\bm{R}_1^{-1}\bm{H}_1\cdot \delta\bm{x}_1 - \bm{\lambda}^T\cdot\delta\bm{x}_1
\end{aligned}
\]
We now have the equation
\[
\begin{aligned}
0 &= \nabla J_1 \cdot\bm{x}\\
&= 2(\bm{x}_0 - \bm{x}_b)^T\bm{B}_0^{-1}\cdot \delta\bm{x}_0 + 2(\bm{x}_1 - \Psi(\bm{x}_0))^T\bm{B}_1^{-1} (\bm{I} \cdot \delta\bm{x}_1+ \Pi_{1;0}^T\cdot\bm{x}_0) \\
&- (\bm{y}_0 -  \bm{H}_0\bm{x}_0)^T\bm{R}_0^{-1}\bm{H}_0\cdot \delta\bm{x}_0 - (\bm{y}_1 - \bm{H}_1\bm{x}_1)^T\bm{R}_1^{-1}\bm{H}_1\cdot \delta\bm{x}_1 - \bm{\lambda}^T\cdot\delta\bm{x}_1.
\end{aligned}
\]

Dividing out differentials and rearranging terms, we see that
\[
\begin{aligned}
\bm{\lambda} &= 2\bm{B}_0^{-T}(\bm{x}_0 - \bm{x}_b) + 2(\bm{I} + \Pi_{1;0}^T)^T\bm{B}_1^{-T}(\bm{x}_1 - \Psi(\bm{x}_0)) \\
&- \bm{H}_0^T\bm{R}_0^{-T}(\bm{y}_0 - \bm{H}_0\bm{x}_0) - \bm{H}_1^T\bm{R}_1^{-T}(\bm{y}_1 - \bm{H}_1\bm{x}_1)
\end{aligned}
\]
The difference between this and the gradient in the notes is that here, we have a term depending on the actual value of $\bm{x}_1$ (instead of the flow map from $\bm{x}_0$ to time $1$), and we only need to compute one $\bm{\lambda}$, instead of two (for two times) because of the constraint that $\bm{x}_1 = \Psi(\bm{x}_0).$


\subsection*{2}
(Note: code attached to the back of the assignment)
\begin{figure}[H]
\includegraphics[scale=0.5]{/Users/zanejakobs/Desktop/4dvarlossr.png}
\end{figure}

\subsection*{3}
Letting $\bm{x} = (x,y)^T$, we have $x_{j+1} = a_j x_j + y_j + \eta_0$, $y_{j+1} = x_j + 2y_j$, and $a_{j+1} = a_j.$ Since $a$ is independent of $x$, differentiating each equation w.r.t. each element of $(x,y,a)$ gives the following Jacobian matrix:
\[
\begin{bmatrix}a & 1 & 0 \\ 1 & 2 & 0 \\ 0 & 0 & 1 \end{bmatrix}
\]
\subsection*{Code}
\begin{Verbatim}
import matplotlib.pyplot as plt
import numpy as np

# x_t -> x_{t+1}
def xmap(x):
    return 3.95 * x * (1 - x)

def psi(x0,t):
    i = 0
    x = x0
    while i < t:
        x = xmap(x)
        i += 1
    return x

def H(x):
    return x + np.random.normal(0, 0.01)


def obs_error(y, x, t):
    xt = psi(x,t)
    return y - H(xt)  

def varobjective4d(x0, y):
    xb = 1./3.
    b0 = 0.1 ** 2

    R = 0.01 ** 2

    J = (1/b0) * (x0 - xb) ** 2 

    for i in range(len(y)):
        e = obs_error(y[i], x0, i)

        J += (1./R) * (e ** 2)

    return J

if __name__ == '__main__':
    
    true_obs = [0.25]
    for i in range(4):
        true_obs.append(xmap(true_obs[-1]))

    obs = [H(x) for x in true_obs]

    Jvals = []

    for i in range(1,len(obs)):
        Jvals.append(varobjective4d(obs[0], obs[:i]))


    plt.plot(Jvals)
    plt.title("4DVAR objective function vs number of data points")
    plt.xlabel("Number of observations")
    plt.ylabel("4DVAR objective")
    plt.show()
\end{Verbatim}




\end{document}